Logic/Modal/Standard/Geach.lean
@@ -73,27 +73,17 @@ instance : IsGeach (α := α) 𝗧𝗰 where taple := ⟨0, 1, 0, 0⟩;
 
 
 def MultiGeach : List Axioms.Geach.Taple → AxiomSet α
-  | [] => 𝗞
+  | [] => ∅
   | x :: xs => (AxiomSet.Geach x) ∪ (AxiomSet.MultiGeach xs)
 notation:max "𝗚𝗲(" l ")" => AxiomSet.MultiGeach l
 
 namespace MultiGeach
 
 @[simp]
-lemma def_nil : 𝗚𝗲([]) = (𝗞 : AxiomSet α) := by simp [MultiGeach]
+lemma def_nil : 𝗚𝗲([]) = (∅ : AxiomSet α) := by simp [MultiGeach]
 
 @[simp]
 lemma iff_cons : 𝗚𝗲(x :: l) = (𝗴𝗲(x) : AxiomSet α) ∪ 𝗚𝗲(l) := by simp only [MultiGeach];
-
-@[simp]
-lemma subsetK : (𝗞 : AxiomSet α) ⊆ 𝗚𝗲(l) := by
-  induction l with
-  | nil => simp;
-  | cons => simp; apply Set.subset_union_of_subset_right (by assumption);
-
-lemma subsetK' (h : 𝗚𝗲(l) ⊆ Ax) : 𝗞 ⊆ Ax := Set.Subset.trans subsetK h
-
--- instance instK : System.K (𝐆𝐞(l) : AxiomSet α) := K_of_subset_K (by simp)
 
 lemma mem (h : x ∈ l) : (𝗴𝗲(x) : AxiomSet α) ⊆ 𝗚𝗲(l) := by
   induction l with
@@ -104,11 +94,19 @@ lemma mem (h : x ∈ l) : (𝗴𝗲(x) : AxiomSet α) ⊆ 𝗚𝗲(l) := by
     . subst_vars; tauto;
     . apply Set.subset_union_of_subset_right $ ih (by assumption);
 
+/-
+@[simp]
+lemma subset_K {l : List Axioms.Geach.Taple} : (𝗞 : AxiomSet α) ⊆ 𝗚𝗲(l) := by
+  induction l with
+  | nil => simp;
+  | cons a as ih => apply Set.subset_union_of_subset_right ih;
+-/
+
+/-
 @[simp]
 lemma subset (h : l₁ ⊆ l₂) : (𝗚𝗲(l₁) : AxiomSet α) ⊆ 𝗚𝗲(l₂) := by
   induction l₁ generalizing l₂ <;> induction l₂;
-  case nil.nil | cons.nil => simp_all;
-  case nil.cons => simp_all; apply Set.subset_union_of_subset_right (by simp);
+  case nil.nil | cons.nil | nil.cons => simp_all;
   case cons.cons a as iha b bs ihb =>
     simp_all;
     constructor;
@@ -116,6 +114,7 @@ lemma subset (h : l₁ ⊆ l₂) : (𝗚𝗲(l₁) : AxiomSet α) ⊆ 𝗚𝗲(l
       . subst_vars; tauto;
       . apply Set.subset_union_of_subset_right $ mem (by assumption);
     . simpa using (iha h.2);
+-/
 
 end MultiGeach
 
@@ -124,17 +123,10 @@ end AxiomSet
 
 namespace DeductionParameter
 
-protected abbrev Geach (l : List Axioms.Geach.Taple) : DeductionParameter α where
-  axiomSet := 𝗚𝗲(l)
-  rules := ⟨true, false, false⟩
+protected abbrev Geach (l : List Axioms.Geach.Taple) : DeductionParameter α := (𝗚𝗲(l))ᴺ
 notation "𝐆𝐞(" l ")" => DeductionParameter.Geach l
-instance instNormal : Normal (α := α) 𝐆𝐞(l) where
-  include_K := by simp [AxiomSet.MultiGeach.subsetK]
 
 namespace Geach
-
-@[simp]
-lemma subset_axm (h : l₁ ⊆ l₂ := by simp_all) : (Ax(𝐆𝐞(l₁)) : AxiomSet α) ⊆ (Ax(𝐆𝐞(l₂)) : AxiomSet α) := by simp_all;
 
 end Geach
 
@@ -144,30 +136,30 @@ protected class IsGeach (L : DeductionParameter α) where
 
 namespace IsGeach
 
-variable {L : DeductionParameter α} [geach : L.IsGeach]
+lemma ax {Λ : DeductionParameter α} [geach : Λ.IsGeach] : Ax(Λ) = (𝗞 ∪ 𝗚𝗲(geach.taples)) := by
+  have e := geach.char;
+  simp [DeductionParameter.Geach] at e;
+  simp_all;
 
-instance : L.Normal := by
+instance {L : DeductionParameter α} [geach : L.IsGeach] : L.IsNormal := by
   rw [geach.char];
-  infer_instance
+  infer_instance;
 
-@[simp]
-lemma eq_axiomset : Ax(L) = 𝗚𝗲(IsGeach.taples L) := by have := geach.char; simp_all;
+instance : 𝐊.IsGeach (α := α) where taples := [];
 
-instance : DeductionParameter.IsGeach (α := α) 𝐊 where taples := [];
+instance : 𝐊𝐃.IsGeach (α := α) where taples := [⟨0, 0, 1, 1⟩]
 
-instance : DeductionParameter.IsGeach (α := α) 𝐊𝐃 where taples := [⟨0, 0, 1, 1⟩]
+instance : 𝐊𝐓.IsGeach (α := α) where taples := [⟨0, 0, 1, 0⟩]
 
-instance : DeductionParameter.IsGeach (α := α) 𝐊𝐓 where taples := [⟨0, 0, 1, 0⟩]
+instance : 𝐒𝟒.IsGeach (α := α) where taples := [⟨0, 0, 1, 0⟩, ⟨0, 2, 1, 0⟩]
 
-instance : DeductionParameter.IsGeach (α := α) 𝐒𝟒 where taples := [⟨0, 0, 1, 0⟩, ⟨0, 2, 1, 0⟩]
+instance : 𝐒𝟒.𝟐.IsGeach (α := α) where taples := [⟨0, 0, 1, 0⟩, ⟨0, 2, 1, 0⟩, ⟨1, 1, 1, 1⟩]
 
-instance : DeductionParameter.IsGeach (α := α) 𝐒𝟒.𝟐 where taples := [⟨0, 0, 1, 0⟩, ⟨0, 2, 1, 0⟩, ⟨1, 1, 1, 1⟩]
+instance : 𝐒𝟓.IsGeach (α := α) where taples := [⟨0, 0, 1, 0⟩, ⟨1, 1, 0, 1⟩]
 
-instance : DeductionParameter.IsGeach (α := α) 𝐒𝟓 where taples := [⟨0, 0, 1, 0⟩, ⟨1, 1, 0, 1⟩]
+instance : 𝐊𝐓𝟒𝐁.IsGeach (α := α) where taples := [⟨0, 0, 1, 0⟩, ⟨0, 2, 1, 0⟩, ⟨0, 1, 0, 1⟩]
 
-instance : DeductionParameter.IsGeach (α := α) 𝐊𝐓𝟒𝐁 where taples := [⟨0, 0, 1, 0⟩, ⟨0, 2, 1, 0⟩, ⟨0, 1, 0, 1⟩]
-
-instance : DeductionParameter.IsGeach (α := α) 𝐓𝐫𝐢𝐯 where taples := [⟨0, 0, 1, 0⟩, ⟨0, 1, 0, 0⟩]
+instance : 𝐓𝐫𝐢𝐯.IsGeach (α := α) where taples := [⟨0, 0, 1, 0⟩, ⟨0, 1, 0, 0⟩]
 
 end IsGeach
 
