Logic/Modal/Standard/Kripke/Dot3.lean
@@ -1,106 +1,85 @@
-import Logic.Modal.Standard.Kripke.Geach.Completeness
+import Logic.Modal.Standard.Kripke.Geach
 
 namespace LO.Modal.Standard
 
+namespace Kripke
+
 open System
 open Kripke
-open Formula Formula.Kripke
+open Formula
 
-variable {α} [Inhabited α] [DecidableEq α]
+abbrev ConnectedFrameClass : FrameClass := { F | Connected F }
 
-variable {F : Kripke.Frame' α}
-variable [atleast : Atleast 2 α]
+variable {α} [Inhabited α] [DecidableEq α] [atleast : Atleast 2 α]
+variable {F : Kripke.Frame}
 
-private lemma AxiomSet.Dot3.definability.implies : F ⊧* .𝟯 → Connected F.Rel := by
+private lemma connected_of_dot3 : F# ⊧* (.𝟯 : AxiomSet α) → Connected F := by
   contrapose;
   intro hCon; simp [Connected] at hCon;
   obtain ⟨x, y, rxy, z, ryz, nryz, nrzy⟩ := hCon;
-  simp [ValidOnFrame];
+  simp [Kripke.ValidOnFrame];
   obtain ⟨f, finv, fInj⟩ := atleast.mapping;
   existsi f 0, f 1, (λ w a =>
     match (finv a) with
     | 0 => y ≺ w
     | 1 => z ≺ w
   );
-  simp [ValidOnModel, not_forall, Axioms.Dot3];
-  existsi x;
+  simp [Kripke.ValidOnModel, Kripke.Satisfies];
+  use x;
   constructor;
-  . existsi y;
+  . use y;
     constructor;
     . assumption;
-    . simp_all [Satisfies, (fInj 0), (fInj 1)];
-  . existsi z;
+    . simp_all [Kripke.Satisfies, (fInj 0), (fInj 1)];
+  . use z;
     constructor;
     . assumption;
-    . simp_all [Satisfies, (fInj 0), (fInj 1)];
+    . simp_all [Kripke.Satisfies, (fInj 0), (fInj 1)];
 
-private lemma AxiomSet.Dot3.definability.impliedBy : Connected F.Rel → F ⊧* .𝟯 := by
+private lemma dot3_of_connected : Connected F → F# ⊧* (.𝟯 : AxiomSet α) := by
   intro hCon;
-  simp [ValidOnFrame, ValidOnModel, Axioms.Dot3];
-  intro _ p q e V x; subst e;
-  simp only [Satisfies.or_def, or_iff_not_imp_left];
-  intro hnxpq;
-  obtain ⟨y, rxy, hyp, hnyq⟩ := by simpa using hnxpq;
-  intro z rxz;
+  simp [Kripke.ValidOnFrame, Kripke.ValidOnModel, Axioms.Dot3];
+  intro δ p q e V x; subst e;
+  simp [Kripke.Satisfies];
+  by_contra hC; push_neg at hC;
+  obtain ⟨⟨y, rxy, hp, hnq⟩, ⟨z, rxz, hq, hnp⟩⟩ := hC;
   cases hCon ⟨rxy, rxz⟩ with
-  | inl ryz =>
-    have := hyp _ ryz;
-    simp_all only [Satisfies.imp_def, implies_true];
-  | inr rzy =>
-    simp [Satisfies.box_def, Satisfies.imp_def]
-    intro hq;
-    have hyp := hq y rzy;
-    contradiction;
+  | inl ryz => exact hnp $ hp ryz;
+  | inr rzy => exact hnq $ hq rzy;
 
-instance AxiomSet.Dot3.definability : Definability (α := α) .𝟯 (λ F => Connected F.Rel) where
-  defines F := by
-    constructor;
-    . exact AxiomSet.Dot3.definability.implies;
-    . exact AxiomSet.Dot3.definability.impliedBy;
+lemma AxDot3_Definability : .𝟯.DefinesKripkeFrameClass (α := α) (ConnectedFrameClass) := by
+  intro F;
+  constructor;
+  . exact connected_of_dot3;
+  . exact dot3_of_connected;
 
-instance S4dot3.definability : Definability (α := α) Ax(𝐒𝟒.𝟑) (λ F => Reflexive F.Rel ∧ Transitive F.Rel ∧ Connected F.Rel) := by
-  have d := Definability.union (P₁ := λ F => (Reflexive F.Rel ∧ Transitive F.Rel)) (by simpa using instGeachDefinability (α := α) (L := 𝐒𝟒)) AxiomSet.Dot3.definability;
-  simp at d;
-  suffices p : ∀ {F : Frame' α}, (Reflexive F.Rel ∧ Transitive F.Rel) ∧ Connected F.Rel ↔ Reflexive F.Rel ∧ Transitive F.Rel ∧ Connected F.Rel by
-    constructor;
-    intro F;
-    constructor;
-    . intro h;
-      apply p.mp;
-      exact d.defines F |>.mp h;
-    . intro h;
-      exact d.defines F |>.mpr $ p.mpr h;
-  aesop;
+abbrev ReflexiveTransitiveConnectedFrameClass : FrameClass := { F | Reflexive F ∧ Transitive F ∧ Connected F }
 
-instance : FiniteFrameClass.IsNonempty (𝔽ꟳ(Ax(𝐒𝟒.𝟑)) : FiniteFrameClass' α) := by
-  existsi Frame.terminal;
-  apply iff_definability_memAxiomSetFrameClass (S4dot3.definability) |>.mpr;
-  refine ⟨?reflexive, ?transitive, ?connective⟩;
-  . intro x; apply Frame.terminal.rel.mpr; trivial;
-  . intro x y z hxy hyz;
-    have := Frame.terminal.rel.mp hxy;
-    have := Frame.terminal.rel.mp hyz;
-    apply Frame.terminal.rel.mpr;
-    tauto;
-  . intro x y z ⟨hxy, hxz⟩;
-    have := Frame.terminal.rel.mp hxy;
-    have := Frame.terminal.rel.mp hxz;
-    subst_vars;
-    left; assumption;
+lemma ReflexiveTransitiveConnectedFrameClass.nonempty : ReflexiveTransitiveConnectedFrameClass.Nonempty.{0} := by
+  use terminalFrame;
+  simp [Reflexive, Transitive, Connected, Frame.Rel'];
 
-instance : FrameClass.IsNonempty (𝔽(Ax(𝐒𝟒.𝟑)) : FrameClass' α) := inferInstance
 
-namespace Kripke
 
-open MaximalConsistentTheory
+private lemma S4Dot3_defines' : (𝗧 ∪ 𝟰 ∪ .𝟯).DefinesKripkeFrameClass (α := α) ReflexiveTransitiveConnectedFrameClass := by
+  rw [(show ReflexiveTransitiveConnectedFrameClass = ({ F | (Reflexive F ∧ Transitive F) ∧ Connected F } : FrameClass) by aesop)];
+  apply AxiomSet.DefinesKripkeFrameClass.union;
+  . exact S4_defines.toAx';
+  . exact AxDot3_Definability;
 
-lemma definability_canonicalFrame_Dot3 {𝓓 : DeductionParameter α} [𝓓.Normal] [Inhabited (𝓓)-MCT] (hAx : .𝟯 ⊆ Ax(𝓓))
-  : Connected (CanonicalFrame 𝓓).Rel := by
+lemma S4Dot3_defines : 𝐒𝟒.𝟑.DefinesKripkeFrameClass (α := α) ReflexiveTransitiveConnectedFrameClass :=
+  DeductionParameter.DefinesKripkeFrameClass.ofAx S4Dot3_defines'
+
+instance : System.Consistent (𝐒𝟒.𝟑 : DeductionParameter α) := consistent_of_defines S4Dot3_defines' ReflexiveTransitiveConnectedFrameClass.nonempty
+
+
+open MaximalConsistentTheory in
+lemma connected_CanonicalFrame {Ax : AxiomSet α} (hAx : .𝟯 ⊆ Ax) [System.Consistent Axᴺ] : Connected (CanonicalFrame Ax) := by
   dsimp only [Connected];
   intro X Y Z ⟨hXY, hXZ⟩;
   by_contra hC; push_neg at hC;
   have ⟨nhYZ, nhZY⟩ := hC; clear hC;
-  simp only [Set.not_subset] at nhYZ nhZY;
+  simp only [Frame.Rel', Set.not_subset] at nhYZ nhZY;
   obtain ⟨p, hpY, hpZ⟩ := nhYZ; replace hpY : □p ∈ Y.theory := hpY;
   obtain ⟨q, hqZ, hqY⟩ := nhZY; replace hqZ : □q ∈ Z.theory := hqZ;
 
@@ -116,28 +95,20 @@ lemma definability_canonicalFrame_Dot3 {𝓓 : DeductionParameter α} [𝓓.Norm
     constructor;
     . assumption;
     . apply iff_mem_imp.not.mpr; simp [hpZ, hqZ];
-  have : (□(□p ⟶ q) ⋎ □(□q ⟶ p)) ∉ X.theory := by
-    apply iff_mem_or.not.mpr; push_neg; exact ⟨hpqX, hqpX⟩;
 
-  have : □(□p ⟶ q) ⋎ □(□q ⟶ p) ∈ X.theory := by
-    apply subset_axiomset _
-    exact hAx (by aesop);
+  have : (□(□p ⟶ q) ⋎ □(□q ⟶ p)) ∉ X.theory := by apply iff_mem_or.not.mpr; push_neg; exact ⟨hpqX, hqpX⟩;
+  have : □(□p ⟶ q) ⋎ □(□q ⟶ p) ∈ X.theory := by apply subset_axiomset _; aesop;
   contradiction;
 
--- MEMO: 冗長すぎる
-instance : Canonical (𝐒𝟒.𝟑 : DeductionParameter α)  := by
-  apply canonical_of_definability S4dot3.definability;
+instance : Complete (𝐒𝟒.𝟑 : DeductionParameter α) (ReflexiveTransitiveConnectedFrameClass#) := instComplete_of_mem_canonicalFrame $ by
   refine ⟨?reflexive, ?transitive, ?connective⟩;
-  . rw [←GeachConfluent.reflexive_def];
-    apply definability_canonicalFrame_GeachAxiom;
-    simp only [AxiomSet.Geach.T_def, Set.subset_tetraunion₂];
+  . simp [←GeachConfluent.reflexive_def];
+    apply geachConfluent_CanonicalFrame;
+    simp [AxiomSet.Geach.T_def];
   . rw [←GeachConfluent.transitive_def];
-    apply definability_canonicalFrame_GeachAxiom;
-    simp only [AxiomSet.Geach.Four_def, Set.subset_triunion₂];
-  . apply definability_canonicalFrame_Dot3;
-    simp only [Set.subset_union_right];
-
-instance : Complete (𝐒𝟒.𝟑 : DeductionParameter α) 𝔽(Ax(𝐒𝟒.𝟑)) := instComplete
+    apply geachConfluent_CanonicalFrame;
+    simp [AxiomSet.Geach.Four_def];
+  . apply connected_CanonicalFrame; simp;
 
 end Kripke
 
