Logic/Modal/Standard/Kripke/GL.lean
@@ -1,0 +1,107 @@
+import Logic.Vorspiel.BinaryRelations
+import Logic.Modal.Standard.Kripke.Soundness
+
+namespace LO.Modal.Standard
+
+namespace Kripke
+
+open System
+open Kripke
+open Formula
+
+variable {α : Type u} [Inhabited α]
+variable {F : Kripke.Frame}
+
+abbrev TransitiveCWFFrameClass : FrameClass := { F | Transitive F ∧ ConverseWellFounded F }
+
+private lemma trans_of_L : F# ⊧* (𝗟 : AxiomSet α) → Transitive F.Rel := by
+  contrapose;
+  intro hT; simp [Transitive] at hT;
+  obtain ⟨w₁, w₂, r₁₂, w₃, r₂₃, nr₁₃⟩ := hT;
+  simp [Kripke.ValidOnFrame, Kripke.ValidOnFrame, Kripke.ValidOnModel, Kripke.Satisfies];
+  use (atom default), (λ w' _ => w' ≠ w₂ ∧ w' ≠ w₃), w₁;
+  constructor;
+  . intro x hx h;
+    by_cases hx₂ : x = w₂;
+    . subst hx₂; simpa [Kripke.Satisfies] using h r₂₃;
+    . by_cases hx₃ : x = w₃ <;> simp_all [Kripke.Satisfies, hx₃];
+  . existsi w₂; simpa [Kripke.Satisfies];
+
+private lemma cwf_of_L  : F# ⊧* (𝗟 : AxiomSet α) → ConverseWellFounded F.Rel := by
+  contrapose;
+  intro hCF;
+  obtain ⟨X, hX₁, hX₂⟩ := by simpa using ConverseWellFounded.iff_has_max.not.mp hCF;
+  simp [Kripke.ValidOnFrame, Kripke.ValidOnFrame, Kripke.ValidOnModel, Kripke.Satisfies];
+  use (atom default), (λ w _ => w ∉ X), hX₁.some;
+  constructor;
+  . intro x _;
+    by_cases hxs : x ∈ X
+    . obtain ⟨y, hy₁, hy₂⟩ := hX₂ x hxs;
+      intro h;
+      exact h (by simp_all only [Kripke.Satisfies]);
+    . aesop;
+  . obtain ⟨w', hw'₁, hw'₂⟩ := hX₂ hX₁.some (by apply Set.Nonempty.some_mem);
+    existsi w';
+    constructor;
+    . simpa using hw'₂;
+    . simpa [Kripke.Satisfies];
+
+private lemma L_of_trans_and_cwf : (Transitive F.Rel ∧ ConverseWellFounded F.Rel) → F# ⊧* (𝗟 : AxiomSet α) := by
+  rintro ⟨hTrans, hWF⟩;
+  simp [AxiomSet.L, Axioms.L];
+  intro p V w;
+  simp [Kripke.Satisfies];
+  contrapose; push_neg;
+  intro h;
+  obtain ⟨z, rwz, hz⟩ := h;
+  obtain ⟨m, ⟨⟨rwm, hm⟩, hm₂⟩⟩ := hWF.has_min ({ x | (F.Rel w x) ∧ ¬(Kripke.Satisfies ⟨F, V⟩ x p) }) (by use z; simp_all)
+  use m;
+  constructor;
+  . exact rwm;
+  . constructor;
+    . simp [flip] at hm₂;
+      intro n rmn;
+      apply not_imp_not.mp $ hm₂ n (hTrans rwm rmn);
+      exact rmn;
+    . exact hm;
+
+lemma axiomL_defines : 𝗟.DefinesKripkeFrameClass (α := α) (TransitiveCWFFrameClass) := by
+  intro F;
+  constructor;
+  . intro h;
+    constructor;
+    . exact trans_of_L h;
+    . exact cwf_of_L h;
+  . exact L_of_trans_and_cwf;
+
+
+abbrev TransitiveIrreflexiveFiniteFrameClass : FiniteFrameClass := { F | Transitive F.toFrame ∧ Irreflexive F.toFrame }
+
+
+lemma TransitiveIrreflexiveFiniteFrameClass.nonempty : TransitiveIrreflexiveFiniteFrameClass.Nonempty.{0} := by
+  use PointFrame;
+  simp [Transitive, Irreflexive];
+
+lemma axiomL_finite_defines : 𝗟.FinitelyDefinesKripkeFrameClass (α := α) TransitiveIrreflexiveFiniteFrameClass := by
+  intro F;
+  constructor;
+  . intro h;
+    obtain ⟨hTrans, hCWF⟩ := axiomL_defines.mp h;
+    refine ⟨hTrans, ?irreflexive⟩;
+    . intro w;
+      simpa using ConverseWellFounded.iff_has_max.mp hCWF {w} (by simp);
+  . intro d;
+    have ⟨hTrans, hIrrefl⟩ := d;
+    apply axiomL_defines.mpr;
+    constructor;
+    . exact hTrans;
+    . exact Finite.converseWellFounded_of_trans_irrefl' F.World_finite hTrans hIrrefl;
+
+instance : Sound (𝐆𝐋 : DeductionParameter α) TransitiveIrreflexiveFiniteFrameClass# := sound_of_finitely_defines axiomL_finite_defines
+
+instance : System.Consistent (𝐆𝐋 : DeductionParameter α) := consistent_of_finitely_defines axiomL_finite_defines TransitiveIrreflexiveFiniteFrameClass.nonempty
+
+
+end Kripke
+
+end LO.Modal.Standard
