Logic/Modal/Standard/Kripke/Geach.lean
@@ -1,0 +1,390 @@
+import Logic.Vorspiel.BinaryRelations
+import Logic.Modal.Standard.Geach
+import Logic.Modal.Standard.Kripke.Completeness
+import Logic.Modal.Standard.Kripke.Reducible
+
+namespace LO.Modal.Standard
+
+open System
+open System.Axioms (Geach)
+
+def GeachConfluent (t : Geach.Taple) (R : α → α → Prop) := ∀ {x y z : α}, (RelItr R t.i x y) ∧ (RelItr R t.j x z) → ∃ u, (RelItr R t.m y u) ∧ (RelItr R t.n z u)
+
+namespace GeachConfluent
+
+variable {R : α → α → Prop}
+
+@[simp]
+lemma serial_def : (GeachConfluent ⟨0, 0, 1, 1⟩ R) ↔ Serial R := by simp [GeachConfluent, Symmetric]; aesop;
+
+@[simp]
+lemma reflexive_def : (GeachConfluent ⟨0, 0, 1, 0⟩ R) ↔ Reflexive R := by simp [GeachConfluent, Reflexive];
+
+@[simp]
+lemma symmetric_def : (GeachConfluent ⟨0, 1, 0, 1⟩ R) ↔ Symmetric R := by simp [GeachConfluent, Symmetric]; aesop;
+
+@[simp]
+lemma transitive_def : (GeachConfluent ⟨0, 2, 1, 0⟩ R) ↔ Transitive R := by simp [GeachConfluent, Transitive]; aesop;
+
+@[simp]
+lemma euclidean_def : (GeachConfluent ⟨1, 1, 0, 1⟩ R) ↔ Euclidean R := by simp [GeachConfluent, Euclidean];
+
+@[simp]
+lemma confluent_def : (GeachConfluent ⟨1, 1, 1, 1⟩ R) ↔ Confluent R := by simp [GeachConfluent, Confluent];
+
+@[simp]
+lemma extensive_def : (GeachConfluent ⟨0, 1, 0, 0⟩ R) ↔ Extensive R := by
+  simp [GeachConfluent, Extensive];
+  constructor;
+  . intro h x y Rxy;
+    have := h rfl Rxy;
+    subst_vars;
+    trivial;
+  . intro h x y z Exy Rxz;
+    have := h Rxz;
+    subst_vars;
+    trivial;
+
+@[simp]
+lemma functional_def : (GeachConfluent ⟨1, 1, 0, 0⟩ R) ↔ Functional R := by simp [GeachConfluent, Functional]; aesop
+
+@[simp]
+lemma dense_def : (GeachConfluent ⟨0, 1, 2, 0⟩ R)  ↔ Dense R := by simp [GeachConfluent, Dense]; aesop;
+
+@[simp]
+lemma satisfies_eq : GeachConfluent (α := α) t (· = ·) := by simp [GeachConfluent];
+
+end GeachConfluent
+
+
+def MultiGeachConfluent (ts : List Geach.Taple) (R : α → α → Prop) : Prop :=
+  match ts with
+  | [] => True
+  | t :: ts => (GeachConfluent t R) ∧ (MultiGeachConfluent ts R)
+
+namespace MultiGeachConfluent
+
+@[simp]
+lemma satisfies_eq : MultiGeachConfluent (α := α) ts (· = ·) := by
+  induction ts <;> simp_all [MultiGeachConfluent];
+
+end MultiGeachConfluent
+
+
+namespace Kripke
+
+variable {α : Type u} [Inhabited α] [DecidableEq α]
+
+
+section
+
+lemma TerminalFrame.geach_confluent : GeachConfluent t (terminalFrame.Rel') := by
+  simp [GeachConfluent];
+  intro x y z Rxy Rxz;
+  replace Rxy := terminalFrame.iff_relItr'.mp Rxy;
+  replace Rxz := terminalFrame.iff_relItr'.mp Rxz;
+  use x; subst_vars;
+  constructor <;> { apply terminalFrame.iff_relItr'.mpr; rfl };
+
+lemma TerminalFrame.multi_geach_confluent : MultiGeachConfluent ts (terminalFrame.Rel') := by
+  induction ts with
+  | nil => simp [MultiGeachConfluent];
+  | cons t ts ih =>
+    simp [MultiGeachConfluent];
+    constructor;
+    . exact TerminalFrame.geach_confluent;
+    . exact ih;
+
+abbrev GeachConfluentFrameClass (t : Geach.Taple) : FrameClass := { F | (GeachConfluent t) F }
+
+lemma GeachConfluentFrameClass.nonempty : (GeachConfluentFrameClass.{0} t).Nonempty := by
+  use terminalFrame
+  exact TerminalFrame.geach_confluent;
+
+
+abbrev MultiGeachConfluentFrameClass (ts : List Geach.Taple) : FrameClass := { F | (MultiGeachConfluent ts) F }
+
+lemma MultiGeachConfluentFrameClass.nonempty : (MultiGeachConfluentFrameClass.{0} ts).Nonempty := by
+  use terminalFrame
+  exact TerminalFrame.multi_geach_confluent;
+
+
+abbrev ReflexiveFrameClass : FrameClass := { F | Reflexive F }
+
+abbrev SerialFrameClass : FrameClass := { F | Serial F }
+
+abbrev ReflexiveEuclideanFrameClass : FrameClass := { F | Reflexive F ∧ Euclidean F }
+
+abbrev EquivalenceFrameClass : FrameClass := { F | Reflexive F ∧ Transitive F ∧ Symmetric F }
+
+abbrev PreorderFrameClass : FrameClass := { F | Reflexive F ∧ Transitive F }
+
+end
+
+section Definability
+
+@[simp]
+lemma MultiGeachConfluentFrameClass.def_nil : MultiGeachConfluentFrameClass [] = AllFrameClass := by rfl;
+
+
+open Formula (atom Kripke.Satisfies)
+open Formula.Kripke.Satisfies (multibox_def multidia_def)
+
+variable [Inhabited α]
+
+lemma axiomGeach_defines : 𝗴𝗲(t).DefinesKripkeFrameClass (α := α) (GeachConfluentFrameClass t) := by
+  intro F;
+  constructor;
+  . rintro h x y z ⟨hi, hj⟩;
+    let M : Model α := { Frame := F, Valuation := λ v _ => y ≺^[t.m] v };
+    simp at h;
+    have him_x : Kripke.Satisfies M x (◇^[t.i](□^[t.m](atom default))) := by
+      apply Kripke.Satisfies.multidia_def.mpr;
+      use y;
+      constructor;
+      . exact hi;
+      . apply Kripke.Satisfies.multibox_def.mpr; aesop;
+    have hjn_x : Kripke.Satisfies M x (□^[t.j](◇^[t.n](atom default))) := h (Formula.atom default) M.Valuation x him_x;
+    have hn_z : Kripke.Satisfies M z (◇^[t.n](atom default)) := Kripke.Satisfies.multibox_def.mp hjn_x hj;
+    obtain ⟨u, hzu, hyu⟩ := Kripke.Satisfies.multidia_def.mp hn_z;
+    use u;
+    exact ⟨hyu, hzu⟩;
+  . simp [AxiomSet.Geach, Axioms.Geach, Kripke.Satisfies];
+    intro h p V x him;
+    apply multibox_def.mpr;
+    intro z rxz;
+    apply multidia_def.mpr;
+    obtain ⟨y, rxy, hbp⟩ := multidia_def.mp him;
+    obtain ⟨u, ryu, rzu⟩ := h ⟨rxy, rxz⟩;
+    use u;
+    constructor;
+    . assumption;
+    . exact (multibox_def.mp hbp) ryu;
+
+
+instance : System.Consistent (𝗴𝗲(t)ᴺ : DeductionParameter α) := consistent_of_defines axiomGeach_defines GeachConfluentFrameClass.nonempty
+
+
+lemma axiomMultiGeach_defines : 𝗚𝗲(ts).DefinesKripkeFrameClass (α := α) (MultiGeachConfluentFrameClass ts) := by
+  induction ts with
+  | nil => simp [AxiomSet.DefinesKripkeFrameClass];
+  | cons t ts ih =>
+    intro F;
+    simp_all only [Semantics.RealizeSet.union_iff, AxiomSet.MultiGeach.iff_cons];
+    constructor;
+    . rintro ⟨ht, hts⟩;
+      constructor;
+      . exact axiomGeach_defines.mp ht;
+      . exact ih.mp hts;
+    . rintro ⟨ht, hts⟩;
+      constructor;
+      . exact axiomGeach_defines.mpr ht;
+      . exact ih.mpr hts;
+
+private def instGeachLogicDefinability
+  {Λ : DeductionParameter α} [geach : Λ.IsGeach]
+  (𝔽 : FrameClass) (h𝔽 : 𝔽 = MultiGeachConfluentFrameClass geach.taples := by simp_all [MultiGeachConfluentFrameClass, MultiGeachConfluent])
+  : Λ.DefinesKripkeFrameClass 𝔽 := by
+  simp [DeductionParameter.DefinesKripkeFrameClass];
+  nth_rw 1 [geach.char];
+  rw [←(Set.univ_inter 𝔽)];
+  rw [h𝔽];
+  exact AxiomSet.DefinesKripkeFrameClass.union axiomK_defines axiomMultiGeach_defines;
+
+lemma S4_defines : 𝐒𝟒.DefinesKripkeFrameClass (α := α) PreorderFrameClass := instGeachLogicDefinability PreorderFrameClass (by
+  simp_all [PreorderFrameClass, PreorderFrameClass];
+  apply Set.eq_of_subset_of_subset <;> simp [MultiGeachConfluent];
+)
+
+
+instance : System.Consistent (𝐆𝐞(ts) : DeductionParameter α) := consistent_of_defines axiomMultiGeach_defines MultiGeachConfluentFrameClass.nonempty
+
+instance {Λ : DeductionParameter α} [geach : Λ.IsGeach] : System.Consistent Λ := by rw [geach.char]; infer_instance;
+
+instance : System.Consistent (𝐒𝟒 : DeductionParameter α) := inferInstance
+
+instance : System.Consistent (𝐒𝟓 : DeductionParameter α) := inferInstance
+
+end Definability
+
+
+section Soundness
+
+private lemma instGeachLogicSoundAux
+  {Λ : DeductionParameter α} [geach : Λ.IsGeach] {𝔽 : FrameClass}
+  (h𝔽 : 𝔽 = MultiGeachConfluentFrameClass geach.taples := by simp_all [MultiGeachConfluentFrameClass, MultiGeachConfluent])
+  : Sound Λ 𝔽# := by
+    rw [geach.char, h𝔽];
+    apply sound_of_defines (α := α) (Ax := 𝗚𝗲(geach.taples));
+    exact axiomMultiGeach_defines;
+
+instance sound_KD : Sound (𝐊𝐃 : DeductionParameter α) SerialFrameClass# := instGeachLogicSoundAux
+
+instance sound_KT : Sound (𝐊𝐓 : DeductionParameter α) ReflexiveFrameClass# := instGeachLogicSoundAux
+
+instance sound_S4 : Sound (𝐒𝟒 : DeductionParameter α) PreorderFrameClass# := instGeachLogicSoundAux
+
+instance sound_S5 : Sound (𝐒𝟓 : DeductionParameter α) ReflexiveEuclideanFrameClass# := instGeachLogicSoundAux
+
+instance sound_KT4B : Sound (𝐊𝐓𝟒𝐁  : DeductionParameter α) EquivalenceFrameClass# := instGeachLogicSoundAux
+
+end Soundness
+
+
+section Completeness
+
+open Theory MaximalConsistentTheory CanonicalFrame
+open DeductionParameter (Normal)
+
+variable {Ax : AxiomSet α} [System.Consistent Axᴺ]
+
+lemma geachConfluent_CanonicalFrame (h : 𝗴𝗲(t) ⊆ Ax) : GeachConfluent t (CanonicalFrame Ax):= by
+  rintro Ω₁ Ω₂ Ω₃ h;
+  have ⟨r₁₂, r₁₃⟩ := h; clear h;
+  have ⟨Ω, hΩ⟩ := lindenbaum (𝓓 := Axᴺ) (T := ((□''⁻¹^[t.m]Ω₂.theory) ∪ (□''⁻¹^[t.n]Ω₃.theory))) $ by
+    apply intro_union_Consistent;
+    intro Γ Δ hΓ hΔ hC;
+
+    replace hΓ : ∀ p ∈ Γ, □^[t.m]p ∈ Ω₂.theory := by simpa using hΓ;
+    have hΓconj : □^[t.m](Γ.conj') ∈ Ω₂.theory := iff_mem_multibox_conj'.mpr hΓ;
+
+    replace hΔ : ∀ p ∈ Δ, □^[t.n]p ∈ Ω₃.theory := by simpa using hΔ;
+    have : □^[t.n](Δ.conj') ∈ Ω₃.theory := iff_mem_multibox_conj'.mpr hΔ;
+
+    have : □^[t.j](◇^[t.n](Γ.conj')) ∈ Ω₁.theory := iff_mem_imp.mp
+      (membership_iff.mpr $ Context.of! $ Normal.maxm! (by aesop))
+      (multiframe_def_multidia.mp r₁₂ hΓconj)
+    have : ◇^[t.n]Γ.conj' ∈ Ω₃.theory := multiframe_def_multibox.mp r₁₃ this;
+
+    have : Axᴺ ⊢! □^[t.n](Δ.conj') ⋏ ◇^[t.n](Γ.conj') ⟶ ⊥ := by
+      apply and_imply_iff_imply_imply'!.mpr;
+      exact imp_trans''!
+        (show Axᴺ ⊢! □^[t.n](Δ.conj') ⟶ □^[t.n](~Γ.conj') by exact imply_multibox_distribute'! $ contra₁'! $ and_imply_iff_imply_imply'!.mp hC)
+        (show Axᴺ ⊢! □^[t.n](~Γ.conj') ⟶ ~(◇^[t.n]Γ.conj') by exact contra₁'! $ and₁'! $ multidia_duality!);
+    have : Axᴺ ⊬! □^[t.n](Δ.conj') ⋏ ◇^[t.n](Γ.conj') ⟶ ⊥ := by simpa using Ω₃.consistent (Γ := [□^[t.n](Δ.conj'), ◇^[t.n](Γ.conj')]) (by simp_all)
+
+    contradiction;
+
+  use Ω; simp only [Set.union_subset_iff] at hΩ;
+  constructor;
+  . apply multiframe_def_multibox.mpr; apply hΩ.1;
+  . apply multiframe_def_multibox.mpr; apply hΩ.2;
+
+lemma multiGeachConfluent_CanonicalFrame (h : 𝗚𝗲(ts) ⊆ Ax) : MultiGeachConfluent ts (CanonicalFrame Ax) := by
+  induction ts with
+  | nil => simp [MultiGeachConfluent];
+  | cons t ts ih =>
+    dsimp only [MultiGeachConfluent];
+    constructor;
+    . apply geachConfluent_CanonicalFrame;
+      simp_all;
+    . apply ih;
+      simp_all;
+
+private instance instMultiGeachComplete : Complete (𝗚𝗲(ts)ᴺ : DeductionParameter α) (MultiGeachConfluentFrameClass ts)# :=
+  instComplete_of_mem_canonicalFrame $ multiGeachConfluent_CanonicalFrame (by rfl)
+
+instance {Λ : DeductionParameter α} [g : Λ.IsGeach] : Complete Λ (MultiGeachConfluentFrameClass g.taples)# := by
+  convert instMultiGeachComplete (α := α);
+  exact g.char;
+
+private def instGeachLogicCompleteAux {Λ : DeductionParameter α} [geach : Λ.IsGeach]
+  {𝔽 : FrameClass.Dep α} (h𝔽 : 𝔽 = MultiGeachConfluentFrameClass geach.taples := by simp_all [MultiGeachConfluentFrameClass, MultiGeachConfluent])
+  : Complete Λ 𝔽 := by
+    convert instMultiGeachComplete (α := α);
+    exact geach.char;
+
+instance : Complete (𝐊𝐓 : DeductionParameter α) (ReflexiveFrameClass#) := instGeachLogicCompleteAux
+
+instance : Complete (𝐒𝟒 : DeductionParameter α) (PreorderFrameClass#) := instGeachLogicCompleteAux
+
+instance : Complete (𝐒𝟓 : DeductionParameter α) (ReflexiveEuclideanFrameClass#) := instGeachLogicCompleteAux
+
+instance : Complete (𝐊𝐓𝟒𝐁 : DeductionParameter α) (EquivalenceFrameClass#) := instGeachLogicCompleteAux
+
+end Completeness
+
+
+section Reducible
+
+
+theorem reducible_KD_KT : (𝐊𝐃 : DeductionParameter α) ≤ₛ 𝐊𝐓 := by
+  apply reducible_of_subset_FrameClass (α := α) SerialFrameClass.{u} ReflexiveFrameClass.{u};
+  simp_all [serial_of_refl];
+
+
+theorem reducible_S4_S5 : (𝐒𝟒 : DeductionParameter α) ≤ₛ 𝐒𝟓 := by
+  apply reducible_of_subset_FrameClass PreorderFrameClass ReflexiveEuclideanFrameClass;
+  simp_all [trans_of_refl_eucl];
+
+theorem equiv_S5_KT4B : (𝐒𝟓 : DeductionParameter α) =ₛ 𝐊𝐓𝟒𝐁 := by
+  apply equiv_of_eq_FrameClass ReflexiveEuclideanFrameClass EquivalenceFrameClass;
+  apply Set.eq_of_subset_of_subset;
+  . simp_all [symm_of_refl_eucl, trans_of_refl_eucl];
+  . simp_all [eucl_of_symm_trans];
+
+
+/- TODO: strict reducible
+theorem LogicalStrictStrong.KD_KT [hα : Nontrivial α] : (𝐊𝐃 : AxiomSet α) <ᴸ 𝐊𝐓 := by
+  constructor;
+  . simp;
+  . obtain ⟨x, y, hxy⟩ := hα.exists_pair_ne
+    simp only [LogicalStrong, not_forall];
+    use (□(Formula.atom default) ⟶ (Formula.atom default));
+    use ⟨Deduction.maxm (by simp)⟩
+    apply not_imp_not.mpr $ AxiomSet.sounds;
+    simp [Formula.FrameClassConsequence];
+    existsi (λ _ w₂ => w₂ = y);
+    constructor;
+    . simp only [AxiomSetFrameClass.geach];
+      apply GeachLogic.frameClassDefinability_aux.mp;
+      simp [Serial];
+    . simp [Formula.FrameConsequence];
+      use (λ w _ => w = y);
+      simp;
+      use x;
+
+theorem LogicalStrictStrong.K4_S4 [hα : Nontrivial α] : (𝐊𝟒 : AxiomSet α) <ᴸ 𝐒𝟒 := by
+  constructor;
+  . apply LogicalStrong.of_subset; simp;
+  . obtain ⟨x, y, hxy⟩ := hα.exists_pair_ne;
+    simp only [LogicalStrong, not_forall];
+    use (□(Formula.atom default) ⟶ (Formula.atom default));
+    use ⟨Deduction.maxm (by simp)⟩
+    apply not_imp_not.mpr $ AxiomSet.sounds;
+    simp [Formula.FrameClassConsequence];
+    existsi (λ _ w₂ => w₂ = y);
+    constructor;
+    . simp only [AxiomSetFrameClass.geach];
+      apply GeachLogic.frameClassDefinability_aux.mp;
+      simp [Transitive];
+    . simp [Formula.FrameConsequence];
+      use (λ w _ => w = y);
+      simp;
+      use x;
+
+theorem LogicalStrictStrong.S4_S5 : (𝐒𝟒 : AxiomSet (Fin 3)) <ᴸ 𝐒𝟓 := by
+  constructor;
+  . simp;
+  . simp only [LogicalStrong, not_forall];
+    existsi (◇(Formula.atom default) ⟶ □◇(Formula.atom default));
+    use ⟨Deduction.maxm (by simp)⟩;
+    apply not_imp_not.mpr $ AxiomSet.sounds;
+    simp [Formula.FrameClassConsequence];
+    existsi (λ w₁ w₂ => (w₁ = w₂) ∨ (w₁ = 0 ∧ w₂ = 1) ∨ (w₁ = 0 ∧ w₂ = 2));
+    constructor;
+    . simp only [AxiomSetFrameClass.geach];
+      apply GeachLogic.frameClassDefinability_aux.mp;
+      simp [Reflexive, Transitive];
+      aesop;
+    . simp [Formula.FrameConsequence];
+      use (λ w₁ w₂ => (w₁ = w₂) ∨ (w₁ = 0 ∧ w₂ = 1) ∨ (w₁ = 0 ∧ w₂ = 2));
+      aesop;
+-/
+
+end Reducible
+
+
+end Kripke
+
+end LO.Modal.Standard
