Logic/Modal/Standard/Kripke/Preservation.lean
@@ -1,0 +1,204 @@
+import Logic.Modal.Standard.Kripke.Semantics
+
+namespace LO.Modal.Standard
+
+variable {α}
+
+namespace Kripke
+
+
+section Bisimulation
+
+structure Model.Bisimulation (M₁ M₂ : Kripke.Model α) where
+  toRel : Rel M₁.World M₂.World
+  atomic {x₁ : M₁.World} {x₂ : M₂.World} {a : α} : toRel x₁ x₂ → ((M₁.Valuation x₁ a) ↔ (M₂.Valuation x₂ a))
+  forth {x₁ y₁ : M₁.World} {x₂ : M₂.World} : toRel x₁ x₂ → x₁ ≺ y₁ → ∃ y₂ : M₂.World, toRel y₁ y₂ ∧ x₂ ≺ y₂
+  back {x₁ : M₁.World} {x₂ y₂ : M₂.World} : toRel x₁ x₂ → x₂ ≺ y₂ → ∃ y₁ : M₁.World, toRel y₁ y₂ ∧ x₁ ≺ y₁
+
+notation M₁ " ⇄ " M₂ => Model.Bisimulation M₁ M₂
+
+instance : CoeFun (Model.Bisimulation M₁ M₂) (λ _ => M₁.World → M₂.World → Prop) := ⟨λ bi => bi.toRel⟩
+
+end Bisimulation
+
+
+section ModalEquivalent
+
+
+def ModalEquivalent (M₁ M₂ : Kripke.Model α) (w₁ : M₁.World) (w₂ : M₂.World) : Prop := ∀ p, w₁ ⊧ p ↔ w₂ ⊧ p
+notation:max "("  M₁ "," w₁ ")" " ↭ " "("  M₂ "," w₂ ")" => ModalEquivalent M₁ M₂ w₁ w₂
+
+open Formula
+
+variable {M₁ M₂ : Kripke.Model α}
+variable (Bi : M₁ ⇄ M₂)
+
+lemma modal_equivalent_of_bisimilar (bisx : Bi x₁ x₂) : (M₁, x₁) ↭ (M₂, x₂) := by
+  intro p;
+  induction p using Formula.rec' generalizing x₁ x₂ with
+  | hatom a => exact Bi.atomic bisx;
+  | hbox p ih =>
+    constructor;
+    . intro h y₂ rx₂y₂;
+      obtain ⟨y₁, ⟨bisy, rx₁y₁⟩⟩ := Bi.back bisx rx₂y₂;
+      exact ih bisy |>.mp (h rx₁y₁);
+    . intro h y₁ rx₁y₁;
+      obtain ⟨y₂, ⟨bisy, rx₂y₂⟩⟩ := Bi.forth bisx rx₁y₁;
+      exact ih bisy |>.mpr (h rx₂y₂);
+  | hand p q ihp ihq =>
+    constructor;
+    . rintro ⟨hp, hq⟩;
+      exact ⟨ihp bisx |>.mp hp, ihq bisx |>.mp hq⟩;
+    . rintro ⟨hp, hq⟩;
+      exact ⟨ihp bisx |>.mpr hp, ihq bisx |>.mpr hq⟩;
+  | hor p q ihp ihq =>
+    constructor;
+    . rintro (hp | hq);
+      . left; exact ihp bisx |>.mp hp;
+      . right; exact ihq bisx |>.mp hq;
+    . rintro (hp | hq);
+      . left; exact ihp bisx |>.mpr hp;
+      . right; exact ihq bisx |>.mpr hq;
+  | himp p q ihp ihq =>
+    constructor;
+    . intro hpq hp;
+      exact ihq bisx |>.mp $ hpq $ ihp bisx |>.mpr hp;
+    . intro hpq hp;
+      exact ihq bisx |>.mpr $ hpq $ ihp bisx |>.mp hp;
+  | _ => simp_all;
+
+end ModalEquivalent
+
+
+section Generation
+
+/-
+class GeneratedSubframe (F F' : Kripke.Frame α) where
+  subset : F'.World ⊆ F.World
+  rel : ∀ {x y : F'.World}, x ≺ y ↔ F.Rel' ⟨x, (by aesop)⟩ ⟨y, (by aesop)⟩ -- MEMO: i.e. F.Rel' = F.Rel' ∪ (F.World × F.World)
+  closed : ∀ {x : F'.World}, ∀ {y : F.World}, ⟨x.1, (by aesop)⟩ ≺ y → y.1 ∈ F'.World
+-/
+
+end Generation
+
+
+section PseudoEpimorphism
+
+variable {δ₁ δ₂}
+
+/-- As known as _p-morphism_. -/
+structure Frame.PseudoEpimorphism (F₁ F₂ : Kripke.Frame) where
+  toFun : F₁.World → F₂.World
+  forth {x y : F₁.World} : x ≺ y → toFun x ≺ toFun y
+  back {w : F₁.World} {v : F₂.World} : toFun w ≺ v → ∃ u, toFun u = v ∧ w ≺ u
+
+infix:80 " →ₚ " => Frame.PseudoEpimorphism
+
+instance : CoeFun (Frame.PseudoEpimorphism F₁ F₂) (λ _ => F₁.World → F₂.World) := ⟨λ f => f.toFun⟩
+
+
+structure Model.PseudoEpimorphism (M₁ M₂ : Kripke.Model α) extends M₁.Frame →ₚ M₂.Frame where
+  atomic {w : M₁.World} {a} : (M₁.Valuation w a) ↔ (M₂.Valuation (toFun w) a)
+
+infix:80 " →ₚ " => Model.PseudoEpimorphism
+
+instance : CoeFun (Model.PseudoEpimorphism M₁ M₂) (λ _ => M₁.World → M₂.World) := ⟨λ f => f.toFun⟩
+
+
+open Formula
+
+variable {F₁ F₂ : Kripke.Frame}
+         {M₁ M₂ : Kripke.Model α}
+         {p : Formula α}
+
+lemma iff_formula_satisfies_morphism (f : M₁ →ₚ M₂) {w : M₁.World}
+  : w ⊧ p ↔ (f w) ⊧ p := by
+  induction p using Formula.rec' generalizing w with
+  | hatom p =>
+    constructor;
+    . apply f.atomic |>.mp;
+    . apply f.atomic |>.mpr
+  | hbox p ih =>
+    constructor;
+    . intro h w₂ hw₂;
+      obtain ⟨w₁, e, hww₁⟩ := f.back hw₂; subst e;
+      exact ih.mp $ h hww₁;
+    . intro h w' hww';
+      exact ih.mpr $ h $ f.forth hww';
+  | _ => simp_all [Kripke.Satisfies];
+
+lemma iff_formula_valid_on_frame_surjective_morphism (f : F₁ →ₚ F₂) (f_surjective : Function.Surjective f) : F₁# ⊧ p → F₂# ⊧ p := by
+  contrapose;
+  intro h;
+  obtain ⟨V₂, w₂, h⟩ := by simpa [Kripke.ValidOnFrame, Kripke.ValidOnModel] using h;
+  simp [Kripke.ValidOnFrame, Kripke.ValidOnModel];
+
+  obtain ⟨w₁, e⟩ := f_surjective w₂; subst e;
+  let V₁ := λ w a => V₂ (f w) a;
+  use V₁, w₁;
+
+  let M₁ : Model α := { Frame := F₁, Valuation := V₁ };
+  let M₂ : Model α := { Frame := F₂, Valuation := V₂ };
+  exact iff_formula_satisfies_morphism (M₁ := M₁) (M₂ := M₂) {
+    toFun := f,
+    forth := f.forth,
+    back := f.back,
+    atomic := by simp_all
+  } |>.not.mpr h;
+
+lemma iff_theory_valid_on_frame_surjective_morphism (f : F₁ →ₚ F₂) (f_surjective : Function.Surjective f) : F₁# ⊧* T → F₂# ⊧* T := by
+  simp only [Semantics.realizeSet_iff];
+  intro h p hp;
+  exact iff_formula_valid_on_frame_surjective_morphism f f_surjective (h hp);
+
+abbrev IrreflexiveFrameClass : FrameClass := { F | Irreflexive F }
+
+theorem undefinable_irreflexive : ¬∃ (Ax : AxiomSet α), AxiomSet.DefinesKripkeFrameClass.{_, 0} Ax IrreflexiveFrameClass := by
+  by_contra hC;
+  obtain ⟨Ax, h⟩ := hC;
+
+  let F₁ : Frame := { World := Fin 2, Rel := (· ≠ ·) };
+  have hIF₁ : Irreflexive F₁ := by simp [Irreflexive, Frame.Rel'];
+
+  let F₂ : Frame := { World := Fin 1, Rel := (· = ·) };
+
+  let f : F₁ →ₚ F₂ := {
+    toFun := λ _ => 0,
+    forth := by simp [Frame.Rel'],
+    back := by
+      simp;
+      intro w;
+      match w with
+      | 0 => use 1;
+      | 1 => use 0;
+  };
+  have f_surjective : Function.Surjective f := by simp [Function.Surjective]; aesop;
+
+  have : ¬Irreflexive F₂ := by simp [Irreflexive];
+  have : Irreflexive F₂ := h.mp $ iff_theory_valid_on_frame_surjective_morphism f f_surjective $ h.mpr hIF₁;
+  contradiction;
+
+
+def Model.PseudoEpimorphism.Bisimulation (f : M₁ →ₚ M₂) : M₁ ⇄ M₂ := {
+  toRel := Function.graph f,
+  atomic := by
+    intro x₁ x₂ a e; subst e;
+    constructor;
+    . apply f.atomic.mp;
+    . apply f.atomic.mpr;
+  forth := by
+    simp;
+    intro x₁ y₁ rx₁y₁;
+    exact f.forth rx₁y₁;
+  back := by
+    simp;
+    intro x₁ x₂ y₂ e rx₂y₂; subst e;
+    obtain ⟨y₁, _⟩ := f.back rx₂y₂;
+    use y₁;
+}
+
+end PseudoEpimorphism
+
+end Kripke
+
+end LO.Modal.Standard
