Logic/Modal/Standard/Kripke/Reducible.lean
@@ -3,42 +3,48 @@ import Logic.Modal.Standard.Kripke.Semantics
 
 namespace LO.Modal.Standard
 
+open DeductionParameter Normal
+
 namespace Kripke
 
-variable
-  {α : Type u} [DecidableEq α]
-  {L₁ L₂ : DeductionParameter α} [L₁.HasNec] [L₂.HasNec]
-  {P₁ P₂ : FrameProperty}
-  [sound₁ : Sound L₁ 𝔽(Ax(L₁))] [sound₂ : Sound L₂ 𝔽(Ax(L₂))]
-  [complete₁ : Complete L₁ 𝔽(Ax(L₁))] [complete₂ : Complete L₂ 𝔽(Ax(L₂))]
-  [definability₁ : Definability Ax(L₁) P₁] [definability₂ : Definability Ax(L₂) P₂]
+open Formula
 
-lemma reducible_of_subset_axiomSetFrameClass (hs : ∀ {F}, F ∈ 𝔽(Ax(L₂)) → F ∈ 𝔽(Ax(L₁))) : L₁ ≤ₛ L₂ := by
+variable {α : Type*} {Ax₁ Ax₂ : AxiomSet α} (𝔽₁ 𝔽₂ : FrameClass)
+  [sound₁ : Sound Ax₁ᴺ 𝔽₁#] [sound₂ : Sound Ax₂ᴺ 𝔽₂#]
+  [complete₁ : Complete Ax₁ᴺ 𝔽₁#] [complete₂ : Complete Ax₂ᴺ 𝔽₂#]
+
+lemma reducible_of_subset_FrameClass (h𝔽 : 𝔽₂ ⊆ 𝔽₁) : Ax₁ᴺ ≤ₛ Ax₂ᴺ := by
   apply System.reducible_iff.mpr;
   intro p hp;
   apply complete₂.complete;
   intro F hF;
-  exact sound₁.sound hp F $ hs hF;
+  exact sound₁.sound hp $ h𝔽 hF;
 
-lemma reducible_of_definability (hs : ∀ {F : Frame}, P₂ F → P₁ F) : L₁ ≤ₛ L₂ := by
-  apply reducible_of_subset_axiomSetFrameClass;
-  intro F hF;
-  apply iff_definability_memAxiomSetFrameClass definability₁ |>.mpr;
-  exact hs $ iff_definability_memAxiomSetFrameClass definability₂ |>.mp hF;
+/-
+lemma strictreducible_of_ssubset_FrameClass (hne : Ax₂.Nonempty) (h𝔽 : 𝔽₂ ⊂ 𝔽₁) : Ax₁ᴺ <ₛ Ax₂ᴺ := by
+  rw [Set.ssubset_def] at h𝔽;
+  constructor;
+  . apply reducible_of_subset_FrameClass sound₁ complete₂; exact h𝔽.1;
+  . apply System.not_reducible_iff.mpr;
+    obtain ⟨p, hp⟩ := hne;
+    use p;
+    constructor;
+    . exact ⟨Deduction.maxm (by simp_all)⟩;
+    . apply (not_imp_not.mpr $ sound₁.sound);
+      simp [Kripke.ValidOnFrameClass];
+      obtain ⟨F, hF₁, hF₂⟩ := by simpa [Set.not_subset] using h𝔽.2;
+      use F;
+      constructor;
+      . exact hF₁;
+      . sorry;
+-/
 
-lemma equiv_of_eq_axiomSetFrameClass
-  (hs₁ : ∀ {F}, F ∈ 𝔽(Ax(L₂)) → F ∈ 𝔽(Ax(L₁)))
-  (hs₂ : ∀ {F}, F ∈ 𝔽(Ax(L₁)) → F ∈ 𝔽(Ax(L₂)))
-  : L₁ =ₛ L₂ := by
+lemma equiv_of_eq_FrameClass (h𝔽 : 𝔽₁ = 𝔽₂) : Ax₁ᴺ =ₛ Ax₂ᴺ := by
   apply System.Equiv.antisymm_iff.mpr;
   constructor;
-  . apply reducible_of_subset_axiomSetFrameClass hs₁;
-  . apply reducible_of_subset_axiomSetFrameClass hs₂;
-
-lemma equiv_of_iff_definability (h : ∀ {F}, P₁ F ↔ P₂ F) : L₁ =ₛ L₂ := by
-  apply System.Equiv.antisymm_iff.mpr;
-  constructor;
-  . apply reducible_of_definability (definability₁ := definability₁) (definability₂ := definability₂); intros; exact h.mpr (by assumption)
-  . apply reducible_of_definability (definability₁ := definability₂) (definability₂ := definability₁); intros; exact h.mp (by assumption)
+  . apply reducible_of_subset_FrameClass 𝔽₁ 𝔽₂;
+    subst_vars; rfl;
+  . apply reducible_of_subset_FrameClass 𝔽₂ 𝔽₁;
+    subst_vars; rfl;
 
 end LO.Modal.Standard.Kripke
