Logic/Modal/Standard/Kripke/Soundness.lean
@@ -3,47 +3,90 @@ import Logic.Modal.Standard.Deduction
 
 namespace LO.Modal.Standard.Kripke
 
-variable {α : Type u}
-         {L : DeductionParameter α} [L.HasNecOnly]
+variable {Ax : AxiomSet α}
 
+open Formula
 open Deduction
-open Formula Formula.Kripke
+open DeductionParameter (Normal)
 
-lemma sound_on_frameclass (d : L ⊢ p) : 𝔽(Ax(L)) ⊧ p := by
-  induction d using Deduction.inducition_with_nec with
-  | hMaxm h => exact validOnAxiomSetFrameClass_axiom h;
-  | hMdp _ _ ihpq ihp =>
-    intro F hF V w;
-    exact Satisfies.mdp (ihpq F hF V w) (ihp F hF V w);
-  | hNec _ ih =>
-    intro F hF V w w' _;
-    exact ih F hF V w';
+section
+
+variable {𝔽 : FrameClass}
+
+lemma sound (defines : Ax.DefinesKripkeFrameClass 𝔽) (d : Axᴺ ⊢! p) : 𝔽# ⊧ p := by
+  induction d using Deduction.inducition_with_necOnly! with
+  | hMaxm h =>
+    simp only [Set.mem_setOf_eq] at h;
+    rcases h with (hK | hR);
+    . exact (Semantics.RealizeSet.setOf_iff.mp Kripke.ValidOnFrameClass.axiomK) _ hK;
+    . intro F hF;
+      exact Semantics.RealizeSet.setOf_iff.mp (defines.mpr hF) _ hR;
+  | hMdp ihpq ihp => exact Kripke.ValidOnFrameClass.mdp ihpq ihp;
+  | hNec ih => exact Kripke.ValidOnFrameClass.nec ih;
   | hDisj₃ =>
-    simp_all [ValidOnFrameClass, ValidOnFrame, ValidOnModel];
+    simp_all [Kripke.ValidOnFrameClass, Kripke.ValidOnFrame, Kripke.ValidOnModel, Kripke.Satisfies];
     intros; rename_i hpr hqr hpq;
     cases hpq with
     | inl hp => exact hpr hp;
     | inr hq => exact hqr hq;
-  | _ => simp_all [ValidOnFrameClass, ValidOnFrame, ValidOnModel];
+  | _ => simp_all [Kripke.ValidOnFrameClass, Kripke.ValidOnFrame, Kripke.ValidOnModel, Kripke.Satisfies];
 
-lemma sound!_on_frameclass : L ⊢! p → 𝔽(Ax(L)) ⊧ p := λ ⟨d⟩ => sound_on_frameclass d
+lemma sound_of_defines (defines : Ax.DefinesKripkeFrameClass 𝔽) : Sound Axᴺ 𝔽# := ⟨sound defines⟩
 
-instance : Sound L 𝔽(L.axiomSet) := ⟨sound!_on_frameclass⟩
+lemma unprovable_bot_of_nonempty_frameClass (defines : Ax.DefinesKripkeFrameClass 𝔽) (nonempty : 𝔽.Nonempty) : Axᴺ ⊬! ⊥ := by
+  by_contra hC;
+  obtain ⟨⟨_, F⟩, hF⟩ := nonempty;
+  simpa using sound defines hC hF;
 
-lemma unprovable_bot [ne : FrameClass.IsNonempty 𝔽(Ax(L))] : L ⊬! ⊥ := by
-  intro h;
-  obtain ⟨F, hF⟩ := ne;
-  simpa using sound!_on_frameclass h F hF;
+lemma consistent_of_defines (defines : Ax.DefinesKripkeFrameClass 𝔽) (nonempty : 𝔽.Nonempty) : System.Consistent Axᴺ := by
+  apply System.Consistent.of_unprovable;
+  exact unprovable_bot_of_nonempty_frameClass defines nonempty;
 
-instance Consistent_of_nonemptyFrameClass [FrameClass.IsNonempty.{u} 𝔽(Ax(L))] : System.Consistent L := System.Consistent.of_unprovable $ unprovable_bot
+instance K_sound : Sound (𝐊 : DeductionParameter α) AllFrameClass# := by simpa [←Normal.isK] using sound_of_defines axiomK_defines;
 
-lemma unprovable_bot_finite [ne : FiniteFrameClass.IsNonempty 𝔽ꟳ(Ax(L))] : L ⊬! ⊥ := by
-  intro h;
-  obtain ⟨F, hF⟩ := ne;
-  simpa using sound!_on_frameclass h F.toFrame hF;
+instance K_consistent' : System.Consistent (𝗞 : AxiomSet α)ᴺ := consistent_of_defines axiomK_defines AllFrameClass.nonempty
 
-instance Consistent_of_nonemptyFiniteFrameClass [FiniteFrameClass.IsNonempty.{u} 𝔽ꟳ(Ax(L))] : System.Consistent L := System.Consistent.of_unprovable $ unprovable_bot_finite
+instance K_consistent : System.Consistent (𝐊 : DeductionParameter α) := by
+  simpa [←Normal.isK] using K_consistent';
 
-instance : System.Consistent (𝐊 : DeductionParameter α) := inferInstance
+end
+
+section
+
+variable {𝔽 : FiniteFrameClass}
+
+lemma finite_sound (defines : Ax.FinitelyDefinesKripkeFrameClass 𝔽) (d : Axᴺ ⊢! p) : (𝔽 : FrameClass)# ⊧ p := by
+  induction d using Deduction.inducition_with_necOnly! with
+  | hMaxm h =>
+    simp only [Set.mem_setOf_eq] at h;
+    rcases h with (hK | hR);
+    . exact (Semantics.RealizeSet.setOf_iff.mp Kripke.ValidOnFrameClass.axiomK) _ hK;
+    . rintro F ⟨FF, hFF, eFF⟩; subst eFF;
+      exact Semantics.RealizeSet.setOf_iff.mp (defines.mpr hFF) _ hR;
+  | hMdp ihpq ihp => exact Kripke.ValidOnFrameClass.mdp ihpq ihp;
+  | hNec ih => exact Kripke.ValidOnFrameClass.nec ih;
+  | hDisj₃ =>
+    simp_all [Kripke.ValidOnFrameClass, Kripke.ValidOnFrame, Kripke.ValidOnModel, Kripke.Satisfies];
+    intros; rename_i hpr hqr hpq;
+    cases hpq with
+    | inl hp => exact hpr hp;
+    | inr hq => exact hqr hq;
+  | _ => simp_all [Kripke.ValidOnFrameClass, Kripke.ValidOnFrame, Kripke.ValidOnModel, Kripke.Satisfies];
+
+lemma sound_of_finitely_defines (defines : Ax.FinitelyDefinesKripkeFrameClass 𝔽) : Sound Axᴺ ↑𝔽# := ⟨finite_sound defines⟩
+
+lemma unprovable_bot_of_nonempty_finite_frameClass (defines : Ax.FinitelyDefinesKripkeFrameClass 𝔽) (nonempty : 𝔽.Nonempty) : Axᴺ ⊬! ⊥ := by
+  by_contra hC;
+  obtain ⟨F, hF⟩ := nonempty;
+  have := @finite_sound α Ax 𝔽 ⊥ defines hC ↑F;
+  simp [FiniteFrameClass.toFrameClass] at this;
+  have := this F hF;
+  contradiction;
+
+lemma consistent_of_finitely_defines (defines : Ax.FinitelyDefinesKripkeFrameClass 𝔽) (nonempty : 𝔽.Nonempty) : System.Consistent Axᴺ := by
+  apply System.Consistent.of_unprovable;
+  exact unprovable_bot_of_nonempty_finite_frameClass defines nonempty;
+
+end
 
 end LO.Modal.Standard.Kripke
