Logic/Modal/Standard/PLoN/Soundness.lean
@@ -6,37 +6,28 @@ namespace PLoN
 
 open Formula
 
-variable {p : Formula α}
+variable {p : Formula α} {Λ : DeductionParameter α}
 
-lemma sound!_on_N (d : 𝐍 ⊢! p) : ℕ𝔽(𝐍) ⊧ p := by
-  induction d using Deduction.inducition! with
-  | hMaxm h => simp at h;
-  | hMdp ihpq ihp =>
-    intro F hF V w;
-    replace ihpq := ihpq F hF V w;
-    replace ihp := ihp F hF V w;
-    exact ihpq ihp;
-  | hNec _ ih =>
-    intro F hF V w w' _;
-    exact ih F hF V w';
-  | hLoeb => simp_all only [Bool.false_eq_true];
-  | hHenkin => simp_all only [Bool.false_eq_true];
-  | hDisj₃ =>
-    simp_all [PLoN_ValidOnFrameClass, PLoN_ValidOnFrame, PLoN_ValidOnModel, PLoN_Satisfies];
-    intros; rename_i hpr hqr hpq;
-    cases hpq with
-    | inl hp => exact hpr hp;
-    | inr hq => exact hqr hq;
-  | _ => simp_all [PLoN_ValidOnFrameClass, PLoN_ValidOnFrame, PLoN_ValidOnModel, PLoN_Satisfies];
+lemma sound (defines : Λ.DefinesPLoNFrameClass 𝔽) (d : Λ ⊢! p) : 𝔽 ⊧ p := by
+  intro F hF;
+  have := defines.mpr hF;
+  exact Semantics.RealizeSet.setOf_iff.mp this p d;
 
-instance : Sound (𝐍 : DeductionParameter α) ℕ𝔽(𝐍) := ⟨sound!_on_N⟩
+lemma sound_of_defines (defines : Λ.DefinesPLoNFrameClass 𝔽) : Sound Λ 𝔽 := ⟨sound defines⟩
 
-lemma unprovable_bot_on_N : (𝐍 : DeductionParameter α) ⊬! ⊥ := by
+lemma unprovable_bot_of_nonempty_frameclass (defines : Λ.DefinesPLoNFrameClass 𝔽) (nonempty : 𝔽.Nonempty) : Λ ⊬! ⊥ := by
   intro h;
-  obtain ⟨F, hF⟩ := FrameClassNonempty.N;
-  simpa using sound!_on_N h F hF;
+  obtain ⟨⟨_, F⟩, hF⟩ := nonempty;
+  simpa using sound defines h hF;
 
-instance : System.Consistent (𝐍 : DeductionParameter α) := System.Consistent.of_unprovable $ unprovable_bot_on_N
+lemma consistent_of_defines (defines : Λ.DefinesPLoNFrameClass 𝔽) (nonempty : 𝔽.Nonempty) : System.Consistent Λ := by
+  apply System.Consistent.of_unprovable;
+  exact unprovable_bot_of_nonempty_frameclass defines nonempty;
+
+
+instance : Sound 𝐍 (AllFrameClass α) := sound_of_defines N_defines
+
+instance : System.Consistent (𝐍 : DeductionParameter α) := consistent_of_defines N_defines AllFrameClass.nonempty
 
 end PLoN
 
