Logic/Vorspiel/BinaryRelations.lean
@@ -82,12 +82,15 @@ section ConverseWellFounded
 lemma ConverseWellFounded.iff_has_max : ConverseWellFounded r ↔ (∀ (s : Set α), Set.Nonempty s → ∃ m ∈ s, ∀ x ∈ s, ¬(r m x)) := by
   simp [ConverseWellFounded, WellFounded.wellFounded_iff_has_min, flip]
 
-variable [Finite α]
-
-lemma Finite.converseWellFounded_of_trans_irrefl [IsTrans α rel] [IsIrrefl α rel] : ConverseWellFounded rel := by
+lemma Finite.converseWellFounded_of_trans_irrefl [Finite α] [IsTrans α rel] [IsIrrefl α rel] : ConverseWellFounded rel := by
   apply @Finite.wellFounded_of_trans_of_irrefl _ _ _
     ⟨by intro a b c rba rcb; exact IsTrans.trans c b a rcb rba⟩
     ⟨by simp [flip, IsIrrefl.irrefl]⟩
+
+lemma Finite.converseWellFounded_of_trans_irrefl' (hFinite : Finite α) (hTrans : Transitive rel) (hIrrefl : Irreflexive rel) : ConverseWellFounded rel :=
+  @Finite.wellFounded_of_trans_of_irrefl _ _ _
+    ⟨by simp [flip]; intro a b c ba cb; exact hTrans cb ba;⟩
+    ⟨by simp [flip]; exact hIrrefl⟩
 
 end ConverseWellFounded
 
